Square 1

code/ecdsap256sha2/Hacl.Impl.LowLevel.fst
@@ -668,6 +668,40 @@ let lemma_320 a b c d u =
     ((pow2 64 - 1) * (pow2 64 - 1)) * pow2 64 * pow2 64 * pow2 64 < pow2 320)
 
 
+val lemma_320_64:a: uint64 -> b: uint64 -> c: uint64 -> d: uint64 -> e: uint64 -> u: uint64 -> Lemma 
+  (uint_v u * uint_v a +  (uint_v u * uint_v b) * pow2 64 + (uint_v u * uint_v c) * pow2 64 * pow2 64 + (uint_v u * uint_v d) * pow2 64 * pow2 64 * pow2 64 + uint_v e  < pow2 320)
+  
+let lemma_320_64 a b c d e u = 
+  assert(uint_v u <= pow2 64 - 1);
+  assert(uint_v a <= pow2 64 - 1);
+  assert(uint_v b <= pow2 64 - 1);
+  assert(uint_v c <= pow2 64 - 1);
+  assert(uint_v d <= pow2 64 - 1);
+  assert(uint_v e <= pow2 64 - 1);
+
+  assert(uint_v u *  uint_v a <= (pow2 64 - 1) * (pow2 64 - 1));
+  assert(uint_v u * uint_v b <= (pow2 64 - 1) * (pow2 64 - 1));
+  assert(uint_v u * uint_v c <= (pow2 64 - 1) * (pow2 64 - 1));
+  assert(uint_v u * uint_v d <= (pow2 64 - 1) * (pow2 64 - 1));
+  
+
+  assert(
+    (uint_v u * uint_v a) +  
+    (uint_v u * uint_v b) * pow2 64 + 
+    (uint_v u * uint_v c) * pow2 64 * pow2 64 + 
+    (uint_v u * uint_v d) * pow2 64 * pow2 64 * pow2 64 + uint_v e <= (
+  (pow2 64 - 1) * (pow2 64 - 1) + 
+  (pow2 64 - 1) * (pow2 64 - 1) * pow2 64 +
+  (pow2 64 - 1) * (pow2 64 - 1) * pow2 64 * pow2 64 + 
+  (pow2 64 - 1) * (pow2 64 - 1) * pow2 64 * pow2 64 * pow2 64 + (pow2 64 - 1)));
+
+  assert_norm((pow2 64 - 1) * (pow2 64 - 1) +  
+    ((pow2 64 - 1) * (pow2 64 - 1)) * pow2 64 + 
+    ((pow2 64 - 1) * (pow2 64 - 1)) * pow2 64 * pow2 64 + 
+    ((pow2 64 - 1) * (pow2 64 - 1)) * pow2 64 * pow2 64 * pow2 64 + (pow2 64 - 1) < pow2 320)
+
+
+
 val sq0: f:  lbuffer uint64 (size 4) -> result: lbuffer uint64 (size 4) -> memory: lbuffer uint64 (size 12) -> temp: lbuffer uint64 (size 5) -> Stack uint64
   (requires fun h -> live h result /\ live h f /\ live h memory /\ live h temp /\ disjoint result temp
     /\ disjoint result memory /\ disjoint memory temp 
@@ -789,12 +823,10 @@ let sq0 f result memory temp =
 
   r
 
-
-
-val sq1: f: felem -> f3: felem -> result: felem -> memory: lbuffer uint64 (size 12) -> 
+val sq1: f: felem -> f4: felem -> result: felem -> memory: lbuffer uint64 (size 12) -> 
   temp: lbuffer uint64 (size 5) -> 
   Stack uint64 
-  (requires fun h -> live h f /\ live h f3 /\ live h result /\ live h temp /\ eq_or_disjoint f3 result /\ disjoint f result /\ live h memory /\ disjoint temp result /\ disjoint memory temp /\ disjoint memory result /\
+  (requires fun h -> live h f /\ live h f4 /\ live h result /\ live h temp /\ eq_or_disjoint f4 result /\ disjoint f4 memory /\ disjoint f4 temp /\ disjoint f result /\ live h memory /\ disjoint temp result /\ disjoint memory temp /\ disjoint memory result /\
   (
     let f = as_seq h f in 
     let f0 = Lib.Sequence.index f 0 in 
@@ -818,11 +850,10 @@ val sq1: f: felem -> f3: felem -> result: felem -> memory: lbuffer uint64 (size 
   (ensures fun h0 c h1 -> modifies (loc result |+| loc memory |+| loc temp) h0 h1 /\
   (
 
-      let f = as_seq h0 f in 
-      let f0 = Lib.Sequence.index f 0 in 
-      let f1 = Lib.Sequence.index f 1 in 
-      let f2 = Lib.Sequence.index f 2 in 
-      let f3 = Lib.Sequence.index f 3 in 
+      let f0 = Lib.Sequence.index (as_seq h0 f) 0 in 
+      let f1 = Lib.Sequence.index (as_seq h0 f) 1  in 
+      let f2 = Lib.Sequence.index (as_seq h0 f) 2 in 
+      let f3 = Lib.Sequence.index (as_seq h0 f) 3 in 
     
       let memory = as_seq h1 memory in 
       let m0 = Lib.Sequence.index memory 0 in 
@@ -841,16 +872,32 @@ val sq1: f: felem -> f3: felem -> result: felem -> memory: lbuffer uint64 (size 
       uint_v m4 + uint_v m5 * pow2 64 == uint_v f0 * uint_v f3 /\
       
       uint_v m6 + uint_v m7 * pow2 64 == uint_v f1 * uint_v f2 /\
-      uint_v m8 + uint_v m9 * pow2 64 == uint_v f1 * uint_v f3
+      uint_v m8 + uint_v m9 * pow2 64 == uint_v f1 * uint_v f3 /\
 
-
-    )
-  
-  
+      as_nat h1 result + uint_v c * pow2 256 = uint_v f1 * as_nat h0 f + as_nat h0 f4
+    ) 
   )
+
+val lemma_320_1: a: nat -> b: nat -> c: nat {c < pow2 64} -> d: nat {d < pow2 256} -> e: nat {e < pow2 256 /\ a + b * pow2 256 = c * d + e}  -> Lemma (b < pow2 64)
+
+let lemma_320_1 a b c d e = 
+  assert_norm ((pow2 64 - 1) * (pow2 256 - 1) + pow2 256 < pow2 320);
+  assert(c <= pow2 64 - 1);
+  assert(d <= pow2 256 - 1);
+  assert(c * d <= (pow2 64 - 1) * (pow2 256 - 1));
+  assert(c * d + e < pow2 320);
+  assert(b * pow2 256 < pow2 320);
+  lemma_div_lt_nat (b * pow2 256) 320 256;
+  assert(((b * pow2 256) / pow2 256) < pow2 64);
+  pow2_multiplication_division_lemma_1 b 256 256;
+  assert((b * pow2 256) / pow2 256 = b);
+  assert(b < pow2 64)
+
 
 let sq1 f f4 result memory tempBuffer = 
   let h0 = ST.get() in 
+  assert_norm (pow2 64 * pow2 64 * pow2 64 * pow2 64 = pow2 256);
+  
   let temp = sub tempBuffer (size 0) (size 1) in 
   let tempBufferResult = sub tempBuffer  (size 1) (size 4) in 
 
@@ -864,43 +911,64 @@ let sq1 f f4 result memory tempBuffer =
   let o2 = sub tempBufferResult (size 2) (size 1) in 
   let o3 = sub tempBufferResult (size 3) (size 1) in 
 
-  let m0 = index memory (size 0) in 
-  
   upd o0 (size 0) (index memory (size 0));
-  let h = index memory (size 1) in 
-  let h1 = ST.get() in 
-
-  assert(uint_v (Lib.Sequence.index (as_seq h1 o0) 0) == uint_v f0 * uint_v f1 - uint_v h * pow2 64);
-
-  
+  let h_0 = index memory (size 1) in 
   mul64 f1 f1 o1 temp;
   let l = index o1 (size 0) in     
-  let c1 = add_carry_u64 (u64 0) l h o1 in 
-  let h = index temp (size 0) in 
+  let c1 = add_carry_u64 (u64 0) l h_0 o1 in 
+  let h_1 = index temp (size 0) in 
 
   mul64 f1 f2 o2 temp;
   let l = index o2 (size 0) in  
   upd memory (size 6) l;
   upd memory (size 7) (index temp (size 0));
+  let c2 = add_carry_u64 c1 l h_1 o2 in
+  let h_2 = index temp (size 0) in   
 
-  let c2 = add_carry_u64 c1 l h o2 in
-  let h = index temp (size 0) in 
-  
+
   mul64 f1 f3 o3 temp;
   let l = index o3 (size 0) in  
   upd memory (size 8) l;
   upd memory (size 9) (index temp (size 0));
+  let c3 = add_carry_u64 c2 l h_2 o3 in
+  let h_3 = index temp (size 0) in 
 
-  let c3 = add_carry_u64 c2 l h o3 in
-  
+    let h6 = ST.get() in 
+    
+  calc (==) {
+    uint_v f1 * as_nat h0 f;
+    (==)
+    {
+      assert(as_nat h0 f ==  uint_v f0 +  uint_v f1 * pow2 64 + uint_v f2 * pow2 64 * pow2 64 + uint_v f3 * pow2 64 * pow2 64 * pow2 64)
+    }
+    uint_v f1 * (uint_v f0 +  uint_v f1 * pow2 64 + uint_v f2 * pow2 64 * pow2 64 + uint_v f3 * pow2 64 * pow2 64 * pow2 64);
+    (==)
+
+    {
+      assert_by_tactic (uint_v f1 * (uint_v f0 +  uint_v f1 * pow2 64 + uint_v f2 * pow2 64 * pow2 64 + uint_v f3 * pow2 64 * pow2 64 * pow2 64) == 
+	uint_v f0 * uint_v f1 +  
+	uint_v f1 * uint_v f1 * pow2 64 + 
+	uint_v f2 * uint_v f1 * pow2 64 * pow2 64 + 
+	uint_v f3 * uint_v f1 * pow2 64 * pow2 64 * pow2 64) canon}
+   as_nat h6 tempBufferResult + (uint_v c3 + uint_v h_3) * (pow2 64 * pow2 64 * pow2 64 * pow2 64);
+   (==)
+   {
+     assert_norm (pow2 64 * pow2 64 * pow2 64 * pow2 64 = pow2 256)
+   }
+
+   as_nat h6 tempBufferResult + (uint_v c3 + uint_v h_3) * pow2 256;
+   };
 
 
-  let temp0 = index temp (size 0) in 
+  let c4 = add4 tempBufferResult f4 result in   
+  let h7 = ST.get() in 
 
-  let c4 = add4 tempBufferResult f4 result in 
-  
-  assume (uint_v c3 + uint_v temp0 + uint_v c4 < pow2 32);
-  c3 +! temp0 +! c4
+  assert_by_tactic (uint_v c4 * pow2 256 + (uint_v c3 + uint_v h_3) * pow2 256 = 
+    (uint_v c4 + uint_v c3 + uint_v h_3) * pow2 256) canon;
+
+  lemma_320_1 (as_nat h7 result) (uint_v c4 + uint_v c3 + uint_v h_3) (uint_v f1) (as_nat h0 f) (as_nat h0 f4);
+
+  c3 +! h_3 +! c4
 
 
 val sq2: f1: felem -> f3: felem -> result: felem  -> memory: lbuffer uint64 (size 12) -> temp: lbuffer uint64 (size 5) -> 
